verify vec_push

theories/typing/lib/vec.v
@@ -8,7 +8,7 @@ Section vec.
   Context `{!typeG Σ}.
 
   Definition freeable_sz' (sz: nat) (l: loc) : iProp Σ :=
-    †{1}l…sz ∨ ⌜Z.of_nat sz = 0⌝.
+    †{1}l…sz ∨ ⌜Z.of_nat sz = 0%Z⌝.
 
   Lemma split_vec_mt {𝔄} l' q d alπ Φ :
     (l' ↦∗{q}: (λ vl, [S(d') := d] ∃(len ex: nat) (l: loc) (aπl: vec (proph 𝔄) len),
@@ -77,7 +77,7 @@ Section vec.
   Next Obligation.
     iIntros (????[|d] tid ?? q ?) "LFT In vec κ //=".
     iDestruct "vec" as (??? aπl[->->]) "(↦tys & ex & †)". iIntros "!>!>!>".
-    iMod (ty_own_proph_mt_big_sepL_v with "LFT In ↦tys κ") as "To↦tys"; [done|].
+    iMod (ty_own_proph_big_sepL_mt_v with "LFT In ↦tys κ") as "To↦tys"; [done|].
     iApply (step_fupdN_wand with "To↦tys"). iIntros "!> >(%&%&%& ξl & To↦tys) !>".
     iExists _, _. iSplit.
     { iPureIntro. rewrite lapply_vapply. by apply proph_dep_constr. }
@@ -195,7 +195,7 @@ Section vec.
     case d; [by iDestruct "bvec" as "[>[] _]"|]=> ?.
     iDestruct "bvec" as "[(%&%&%& big) †]".
     iMod (bi.later_exist_except_0 with "big") as (?) "(>-> & >↦ & >↦' & >↦'' & big)".
-    wp_read. wp_op. wp_read. do 3 wp_op. wp_read. rewrite leak_mt_big_sepL.
+    wp_read. wp_op. wp_read. do 3 wp_op. wp_read. rewrite leak_big_sepL_mt_ty_own.
     iDestruct "big" as "((%& %Eq & ↦len) & (%& %Eq' & ↦ex) & †')".
     wp_bind (delete _). iApply (wp_delete _ _ _ (_ ++ _) with "[↦len ↦ex †']").
     { rewrite app_length -Nat2Z.inj_add -Nat2Z.inj_mul Nat.mul_add_distr_r.
@@ -259,6 +259,109 @@ Section vec.
       by rewrite iEq -vlookup_lookup -vapply_lookup=> <-.
   Qed.
 
+  Definition vec_push {𝔄} (ty: type 𝔄) : val :=
+    fn: ["v"; "x"] :=
+      let: "v'" := !"v" in delete [ #1; "v"];;
+      let: "len" := !"v'" in let: "ex" := !("v'" +ₗ #1) in "v'" <- "len";;
+      "v'" <- "len" + #1;;
+      withcont: "push":
+        if: "ex" ≤ #0 then
+          "v'" +ₗ #1 <- "len";; let: "l" := !("v'" +ₗ #2) in
+          let: "l'" := new [(#2 * "len" + #1) * #ty.(ty_size)] in
+          memcpy ["l'"; "len" * #ty.(ty_size); "l"];;
+          delete ["len" * #ty.(ty_size); "l"];;
+          "v'" +ₗ #2 <- "l'";; "push" []
+        else
+          "v'" +ₗ #1 <- "ex" - #1;; "push" []
+      cont: "push" [] :=
+        !("v'" +ₗ #2) +ₗ "len" * #ty.(ty_size) <-{ty.(ty_size)} !"x";;
+        delete [ #ty.(ty_size); "x"];;
+        let: "r" := new [ #0] in return: ["r"].
+
+  Lemma vec_push_type {𝔄} (ty: type 𝔄) :
+    typed_val (vec_push ty) (fn<α>(∅; &uniq{α} (vec_ty ty), ty) → ())
+      (λ post '-[(al, al'); a], al' = al ++ [a] → post ()).
+  Proof.
+    eapply type_fn; [solve_typing|]=> α ??[v[x[]]]. simpl_subst.
+    iIntros (tid(vπ & aπ &[])?) "#LFT #TIME #PROPH #UNIQ #E Na L C /=(v & x &_) #Obs".
+    rewrite !tctx_hasty_val. iDestruct "v" as ([|dv]) "[_ v]"=>//.
+    case v as [[|v|]|]=>//. iDestruct "v" as "[(%vl & >↦ & [#LftIn uniq]) †]".
+    case vl as [|[[|v'|]|][]]; try by iDestruct "uniq" as ">[]".
+    iDestruct "x" as ([|dx]) "[⧖x x]"=>//. case x as [[|x|]|]=>//.
+    rewrite heap_mapsto_vec_singleton. wp_read. wp_let. wp_bind (delete _).
+    rewrite -heap_mapsto_vec_singleton freeable_sz_full.
+    iApply (wp_persistent_time_receipt with "TIME ⧖x"); [done|].
+    iApply (wp_delete _ with "[$↦ $†]"); [done|]. iIntros "!>_ ⧖x".
+    iDestruct "uniq" as (du i [? Eq2]) "[Vo Bor]".
+    move: Eq2. set ξ := PrVar _ i=> Eq2.
+    iMod (lctx_lft_alive_tok α with "E L") as (?) "(α & L & ToL)"; [solve_typing..|].
+    iMod (bor_acc with "LFT Bor α") as "[(%&%& ↦vec & ⧖u & Pc) ToBor]"; [done|].
+    wp_seq. iDestruct (uniq_agree with "Vo Pc") as %[<-<-].
+    rewrite split_vec_mt. case du as [|du]=>//.
+    iDestruct "↦vec" as (len ex ? aπl Eq1) "(↦₀ & ↦₁ & ↦₂ & ↦tys & (%wl &%& ↦ex) & †)".
+    wp_read. wp_let. wp_op. wp_read. wp_let. wp_write. wp_op. wp_write.
+    have ->: (len + 1)%Z = S len by lia.
+    iCombine "⧖u ⧖x" as "#⧖"=>/=. set d := du `max` dx.
+    iMod (uniq_update with "UNIQ Vo Pc") as "[Vo Pc]"; [done|].
+    set push := (rec: "push" _ := _)%E.
+    iAssert (
+      (∃(ex: nat) (l: loc), v' ↦ #(S len) ∗ (v' +ₗ 1) ↦ #ex ∗ (v' +ₗ 2) ↦ #l ∗
+        ([∗ list] i ↦ aπ ∈ aπl, (l +ₗ[ty] i) ↦∗: ty.(ty_own) aπ du tid) ∗
+        (l +ₗ[ty] len) ↦∗len (S ex * ty.(ty_size)) ∗
+        freeable_sz' ((S len + ex) * ty.(ty_size)) l) -∗
+      WP push [] {{ _, cont_postcondition }})%I
+      with "[L ToL Na C Vo Pc ToBor x]" as "push".
+    { iIntros "/=(%ex' &%& ↦₀ & ↦₁ & ↦₂ & ↦tys & (%vl & %Len & ↦ex) & †)".
+      rewrite /push. wp_rec. wp_op. wp_read. do 2 wp_op. wp_bind (_ <-{_} !_)%E.
+      move: {Len}(app_length_ex vl _ _ Len)=> [vl'[?[->[Len ?]]]].
+      rewrite heap_mapsto_vec_app shift_loc_assoc_nat Len -Nat2Z.inj_mul.
+      iDestruct "↦ex" as "[↦ ↦ex]". iDestruct "x" as "[(%& ↦x & ty) †x]".
+      iDestruct (ty_size_eq with "ty") as %Sz. rewrite freeable_sz_full.
+      iApply (wp_memcpy with "[$↦ $↦x]"); [lia..|]. iIntros "!> [↦ ↦x]". wp_seq.
+      wp_bind (delete _). iApply (wp_delete with "[$↦x †x]"); [lia|by rewrite Sz|].
+      iIntros "!>_". wp_seq. set vπ' := λ π, (lapply (vsnoc aπl aπ) π, π ξ).
+      iMod ("ToBor" with "[↦₀ ↦₁ ↦₂ ↦tys ↦ ty ↦ex † Pc]") as "[Bor α]".
+      { iNext. iExists _, _. rewrite split_vec_mt. iFrame "⧖ Pc".
+        iExists _, _, _, (vsnoc aπl _). iFrame "↦₀ ↦₁ ↦₂ †". iSplit; [done|].
+        iSplitR "↦ex"; last first. { iExists _. rewrite/= plus_comm. by iFrame. }
+        iNext. rewrite vsnoc_list big_sepL_app. iSplitL "↦tys".
+        { iClear "#". iStopProof. do 6 f_equiv. apply ty_own_depth_mono. lia. }
+        rewrite/= right_id. iExists _. rewrite vec_to_list_length Nat.add_0_r.
+        iFrame "↦". iApply ty_own_depth_mono; [|done]. lia. }
+      iMod ("ToL" with "α L") as "L".
+      iApply (type_type +[#v' ◁ &uniq{α} (vec_ty ty)] -[vπ']
+        with "[] LFT TIME PROPH UNIQ E Na L C [-] []").
+      - iApply type_new; [done|]. intro_subst.
+        iApply type_jump; [solve_typing|solve_extract|solve_typing].
+      - rewrite/= right_id (tctx_hasty_val #_). iExists _.
+        iFrame "⧖ LftIn". iExists _, _.
+        rewrite (proof_irrel (@prval_to_inh' (listₛ 𝔄) vπ')
+          (@prval_to_inh' (listₛ 𝔄) vπ)). by iFrame.
+      - iApply proph_obs_impl; [|done]=> π.
+        move: (equal_f Eq1 π) (equal_f Eq2 π)=>/=. case (vπ π)=>/= ??->-> Imp Eq.
+        apply Imp. move: Eq. by rewrite vsnoc_list lapply_app. }
+    rewrite /push. wp_let. wp_op. wp_case. case ex as [|ex']=>/=; last first.
+    { do 2 wp_op. have ->: (S ex' - 1)%Z = ex' by lia. wp_write.
+      iApply "push". iExists _, _. iFrame "↦tys ↦₀ ↦₁ ↦₂".
+      iSplitL "↦ex". { iExists _. iFrame. iPureIntro. lia. }
+      iClear "#". iStopProof. f_equiv. lia. }
+    wp_op. wp_write. wp_op. wp_read. wp_let. do 3 wp_op. wp_bind (new _).
+    iApply wp_new; [lia|done|]. iIntros "!>" (?) "[†' ↦']". wp_let. wp_op.
+    have ->: ∀sz: nat, ((2 * len + 1) * sz)%Z = (len + S len) * sz by lia.
+    rewrite split_big_sepL_mt_ty_own plus_0_r Nat2Z.id Nat.mul_add_distr_r
+      repeat_app heap_mapsto_vec_app.
+    iDestruct "↦tys" as (?) "[↦ tys]". iDestruct "↦'" as "[↦' ↦ex']".
+    iDestruct (big_sepL_ty_own_length with "tys") as %Len. wp_bind (memcpy _).
+    iApply (wp_memcpy with "[$↦' $↦]"); [rewrite repeat_length; lia|lia|].
+    iIntros "!>[↦' ↦]". wp_seq. wp_op. rewrite -Nat2Z.inj_mul. wp_bind (delete _).
+    iApply (wp_delete with "[$↦ †]"); [lia|by rewrite Len|]. iIntros "!>_".
+    wp_seq. wp_op. wp_write. iApply "push". iExists _, _. iFrame "↦₀ ↦₁ ↦₂".
+    iSplitL "↦' tys". { rewrite split_big_sepL_mt_ty_own. iExists _. iFrame. }
+    iSplitR "†'".
+    - iExists _. rewrite repeat_length. iFrame "↦ex'". by rewrite repeat_length.
+    - by have <-: ∀sz, sz + (len + len) * sz = len * sz + (sz + len * sz) by lia.
+  Qed.
+
   Local Lemma lapply_app_vinitlast {A B n} (fl: vec (B → A) (S n)) x al a :
     lapply fl x = al ++ [a] → al = lapply (vinit fl) x ∧ a = vlast fl x.
   Proof.
@@ -284,10 +387,10 @@ Section vec.
   Proof.
     eapply type_fn; [solve_typing|]=> α ??[v[]]. simpl_subst.
     iIntros (?[vπ[]]?) "#LFT TIME #PROPH #UNIQ #E Na L C /=[v _] #Obs".
-    rewrite tctx_hasty_val. iDestruct "v" as ([|]) "[_ box]"=>//.
-    case v as [[|v|]|]=>//. iDestruct "box" as "[(%vl & >↦ & [#LftIn uniq]) †]".
+    rewrite tctx_hasty_val. iDestruct "v" as ([|]) "[_ v]"=>//.
+    case v as [[|v|]|]=>//. iDestruct "v" as "[(%vl & >↦ & [#LftIn uniq]) †]".
     case vl as [|[[|v'|]|][]]; try by iDestruct "uniq" as ">[]".
-    rewrite heap_mapsto_vec_singleton. wp_read. wp_seq. wp_bind (delete _).
+    rewrite heap_mapsto_vec_singleton. wp_read. wp_let. wp_bind (delete _).
     rewrite -heap_mapsto_vec_singleton freeable_sz_full.
     iApply (wp_delete _ with "[$↦ $†]"); [done|]. iIntros "!>_".
     iDestruct "uniq" as (d i [? Eq2]) "[Vo Bor]".
@@ -297,9 +400,9 @@ Section vec.
     wp_seq. iDestruct (uniq_agree with "Vo Pc") as %[<-<-].
     rewrite split_vec_mt. case d=>// ?.
     iDestruct "↦vec" as (? ex ? aπl Eq1) "(↦₀ & ↦₁ & ↦₂ & ↦tys & (%wl &%& ↦ex) & †)".
-    wp_read. wp_seq. wp_op. wp_read. wp_seq. wp_op. wp_seq. wp_write.
+    wp_read. wp_let. wp_op. wp_read. wp_let. wp_op. wp_let. wp_write.
     do 2 wp_op. wp_write. wp_bind (new _). iApply wp_new; [lia|done|].
-    iIntros "!>" (r) "[†r ↦r]". rewrite Nat2Z.id. wp_seq. wp_op. wp_read. do 2 wp_op.
+    iIntros "!>" (r) "[†r ↦r]". rewrite Nat2Z.id. wp_let. wp_op. wp_read. do 2 wp_op.
     iMod (proph_obs_sat with "PROPH Obs") as %[π' Obs]; [done|].
     move: Obs (equal_f Eq1 π')=>/=. case (vπ π')=>/= ??[?[?[-> _]]] /(f_equal length).
     rewrite last_length. case aπl as [|aπ len' aπl]=>// _.
